made them modules instead of sections

Coherence.v
@@ -1,230 +1,34 @@
+Require Import Orders OrdersTac.
 Set Implicit Arguments.
 
-Record Coherence t :=
-  { slt: t -> t -> Prop;
+Module Type Coherence.
+  Parameter t : Type.
+  Parameter eq : t -> t -> Prop.
+  Parameter eq_equiv : Equivalence eq.
+  Parameter lt : t -> t -> Prop.
+  Parameter lt_strorder : StrictOrder lt.
+  Parameter lt_compat : Proper (eq ==> eq ==> iff) lt.
+  Parameter le : t -> t -> Prop.
+  Parameter le_lteq : forall x y : t, le x y <-> lt x y \/ eq x y.
+  Parameter lt_total : forall x y : t, lt x y \/ eq x y \/ lt y x.
 
-    slt_irrefl: forall x, ~ slt x x;
-    slt_trans: forall x y z, slt x y -> slt y z -> slt x z;
+  Parameter Mo Sh In: t.
+  Parameter ub_Mo: forall x, lt Mo x -> False.
+  Parameter lb_In: forall x, lt x In -> False.
 
-    slt_total: forall x y, slt x y \/ x = y \/ slt y x;
+  Parameter compatible: t -> t -> Prop.
 
-    Mo: t;
-    Sh: t;
-    In: t;
+  Parameter compatible_prop: forall x1 x2 y1 y2, compatible x1 y1 ->
+                                                 le x2 x1 -> le y2 y1 ->
+                                                 compatible x2 y2.
 
-    ub_Mo: forall x, slt Mo x -> False;
-    lb_In: forall x, slt x In -> False;
+  Parameter ne_In_Sh: ~ eq In Sh.
+  Parameter ne_In_Mo: ~ eq In Mo.
+  Parameter ne_Sh_Mo: ~ eq Sh Mo.
 
-    compatible: t -> t -> Prop;
+  Hint Resolve ub_Mo lb_In compatible_prop ne_In_Sh ne_In_Mo ne_Sh_Mo.
+End Coherence.
 
-    compatible_prop: forall x1 x2 y1 y2, compatible x1 y1 ->
-                                         (slt x1 x2 \/ x1 = x2) -> (slt y1 y2 \/ y1 = y2) ->
-                                         compatible x2 y2;
-
-    ne_In_Sh: In <> Sh;
-    ne_In_Mo: In <> Mo;
-    ne_Sh_Mo: Sh <> Mo
-  }.
-
-Section CoherenceFacts.
-  Variable t: Type.
-  Variable ord: Coherence t.
-
-  Definition sle x y := slt ord x y \/ x = y.
-
-  Theorem sle_refl x: sle x x.
-  Proof.
-    unfold sle; intuition.
-  Qed.
-
-  Theorem slt_asym x y: slt ord x y -> slt ord y x -> False.
-  Proof.
-    pose proof (slt_trans ord x y x).
-    pose proof (slt_irrefl ord x).
-    intuition.
-  Qed.
-
-  Theorem sle_antisym x y: sle x y -> sle y x -> x = y.
-  Proof.
-    pose proof (slt_asym x y).
-    unfold sle; intuition.
-  Qed.
-
-  Theorem neq_sym (x y: t): x <> y -> y <> x.
-  Proof.
-    intuition.
-  Qed.
-
-  Theorem sle_trans x y z: sle x y -> sle y z -> sle x z.
-  Proof.
-    pose proof (slt_trans ord x y z).
-    unfold sle; intuition; match goal with
-                             | H: ?x = ?y |- _ => rewrite H in *; clear H
-                             | _ => idtac
-                           end; intuition.
-  Qed.
-
-  Theorem sle_slt_trans x y z: sle x y -> slt ord y z -> slt ord x z.
-  Proof.
-    pose proof (slt_trans ord x y z).
-    unfold sle; intuition; match goal with
-                             | H: ?x = ?y |- _ => rewrite H in *; clear H
-                             | _ => idtac
-                           end; intuition.
-  Qed.
-
-  Theorem slt_sle_trans x y z: slt ord x y -> sle y z -> slt ord x z.
-  Proof.
-    pose proof (slt_trans ord x y z).
-    unfold sle; intuition; match goal with
-                             | H: ?x = ?y |- _ => rewrite H in *; clear H
-                             | _ => idtac
-                           end; intuition.
-  Qed.
-
-  Lemma slt_neq x y: slt ord x y -> x <> y.
-  Proof.
-    intros f s; rewrite <- s in *.
-    pose proof (slt_irrefl ord x); intuition.
-  Qed.
-
-  Theorem not_neq_eq (x y: t): ~ x <> y -> x = y.
-  Proof.
-    intros.
-    pose proof (@slt_neq x y).
-    pose proof (@slt_neq y x).
-    destruct (slt_total ord x y); intuition.
-  Qed.
-
-  Theorem not_sge_slt x y: ~ sle y x -> slt ord x y.
-  Proof.
-    unfold sle in *.
-    pose proof (slt_irrefl ord x).
-    pose proof (slt_irrefl ord y).
-    pose proof (slt_total ord x y).
-    pose proof (slt_total ord y x).
-    try match goal with
-          | H: ?x = ?y |- _ => rewrite H; clear H
-        end; intuition.
-  Qed.
-
-  Theorem not_sgt_sle x y: ~ slt ord y x -> sle x y.
-  Proof.
-    unfold sle in *.
-    pose proof (slt_irrefl ord x).
-    pose proof (slt_irrefl ord y).
-    pose proof (slt_total ord x y).
-    pose proof (slt_total ord y x).
-    try match goal with
-          | H: ?x = ?y |- _ => rewrite H; clear H
-        end; intuition.
-  Qed.
-
-  Theorem sle_neq_slt x y: sle x y -> x <> y -> slt ord x y.
-  Proof.
-    unfold sle in *.
-    intuition.
-  Qed.
-
-  Lemma ne_Sh_In: Sh ord <> In ord.
-  Proof.
-    pose proof (ne_In_Sh ord).
-    unfold not; let X := fresh in intros X; rewrite X in *; intuition.
-  Qed.
-
-  Lemma ne_Mo_In: Mo ord <> In ord.
-  Proof.
-    pose proof (ne_In_Mo ord).
-    unfold not; let X := fresh in intros X; rewrite X in *; intuition.
-  Qed.
-
-  Lemma ne_Mo_Sh: Mo ord <> Sh ord.
-  Proof.
-    pose proof (ne_Sh_Mo ord).
-    unfold not; let X := fresh in intros X; rewrite X in *; intuition.
-  Qed.
-
-  Definition sgt x y := slt ord y x.
-  Definition sge x y := sle y x.
-End CoherenceFacts.
-
-Ltac order_prepare ord :=
-  unfold not in *;
-  match goal with
-    | H: context [slt _ ?x ?y \/ ?x = ?y] |- _ => fold (sle ord x y) in H; order_prepare
-    | |- context [slt _ ?x ?y \/ ?x = ?y] => fold (sle ord x y); order_prepare
-    | H: slt _ ?x ?y -> False |- _ => apply (not_sgt_sle ord y x) in H; order_prepare
-    | H: sle _ ?x ?y -> False |- _ => apply (not_sge_slt ord y x) in H; order_prepare
-    | |- ?x = ?x => reflexivity
-    | |- sle _ ?x ?x => apply (sle_refl ord x)
-    | _ => (apply not_neq_eq; intro) ||
-           (apply not_sge_slt; intro) ||
-           (apply not_sgt_sle; intro) || exfalso
-  end.
-
-Ltac order_loop ord :=
-  match goal with
-    | H: slt _ ?x ?x |- _ => apply (slt_irrefl ord x H)
-    | H: ?x <> ?x |- _ => exact (H (eq_refl x))
-    | H: sle _ ?x ?x |- _ => clear H; order_loop ord
-    | H: ?x = ?y |- _ => rewrite H in *; order_loop ord
-
-    | H1: sle _ ?x ?y, H2: sle _ ?y ?x |- _ =>
-        generalize (sle_antisym H1 H2); clear H1 H2; intro; order_loop ord
-
-    | H1: sle _ ?x ?y, H2: ?x <> ?y |- _ =>
-        generalize (sle_neq_slt H1 H2); clear H1 H2; intro; order_loop ord
-    | H1: sle _ ?x ?y, H2: ?y <> ?x |- _ =>
-        generalize (sle_neq_slt H1 (neq_sym H2)); clear H1 H2; intro; order_loop ord
-    | H1 : slt _ ?x ?y, H2 : slt _ ?y ?z |- _ =>
-        match goal with
-          | H : slt _ x z |- _ => fail 1
-          | _ => generalize (slt_trans ord x y z H1 H2); intro; order_loop ord
-        end
-    | H1 : sle _ ?x ?y, H2 : slt _ ?y ?z |- _ =>
-       match goal with
-         | H : slt _ x z |- _ => fail 1
-         | _ => generalize (sle_slt_trans z H1 H2); intro; order_loop ord
-       end
-    | H1 : slt _ ?x ?y, H2 : sle _ ?y ?z |- _ =>
-       match goal with
-         | H : slt _ x z |- _ => fail 1
-         | _ => generalize (slt_sle_trans H1 H2); intro; order_loop ord
-       end
-    | H1: sle _ ?x ?y, H2 : sle _ ?y ?z |- _ =>
-       match goal with
-         | H : sle _ x z |- _ => fail 1
-         | _ => generalize (sle_trans H1 H2); intro; order_loop ord
-       end
-    | _ => idtac
-   end.
-
-Hint Resolve ub_Mo lb_In.
-
-Ltac order ord :=
-  pose proof (ne_In_Sh ord);
-  pose proof (ne_In_Mo ord);
-  pose proof (ne_Sh_Mo ord);
-  pose proof (ne_Sh_In ord);
-  pose proof (ne_Mo_In ord);
-  pose proof (ne_Mo_Sh ord);
-  unfold sgt, sge in *; unfold not; intros; order_prepare ord; order_loop ord; auto; fail "Order tactic failed".
-
-Section Test.
-  Variable t: Type.
-  Variable ord: Coherence t.
-  Theorem test1 x y: slt ord x y -> ~ slt ord y x.
-  Proof.
-    order ord.
-  Qed.
-
-  Theorem test2 x: ~ slt ord (Mo ord) x.
-  Proof.
-    eauto.
-  Qed.
-
-  Theorem test3 x: ~ slt ord x (In ord).
-  Proof.
-    eauto.
-  Qed.
-End Test.
+Module CoherenceSolve (cb: Coherence).
+  Include !MakeOrderTac cb cb.
+End CoherenceSolve.
