FirstLevel.v
@@ -2,167 +2,139 @@ Require Import StoreAtomicity Coherence CacheLocal Tree DataTypes Case Useful.
 
 Set Implicit Arguments.
 
-Ltac expandCl cl :=
-  destruct cl as [getCacheState respFn stateZero dirZero dataZero
-                  waitZero dwaitZero nextZero respFnIdx respFnLdData];
-  simpl in *.
-
-Section FirstLevel.
-  Variable State: Set.
-  Variable coh: Coherence State.
-
-  Variable cl: CacheLocal coh.
-
-  Definition s t := getCacheState cl t.
-  Definition nextS t := getCacheState cl (S t).
-
+Module Type FirstLevel (Import coh: Coherence) (Import cl: CacheLocal coh).
   Definition clean a t p :=
-    sle coh (Sh coh) (state (s t) p a) /\ forall c, parent c p -> sle coh (dir (s t) p c a) (Sh coh).
+    le Sh (state t p a) /\ forall c, parent c p -> le (dir t p c a) Sh.
 
-  Ltac expandFl fl :=
-    destruct fl as [latestValue processReq nextChange noReqAgain];
-    unfold clean, s, nextS in *.
+  Definition noStoreData d a t :=
+    d = initData a /\ forall t', t' < t -> noStore respFn t' a.
 
-  Ltac expandClFl cl fl :=
-    expandFl fl;
-    expandCl cl.
+  Definition isStoreData d a t :=
+    exists tm, tm < t /\ match respFn tm with
+                           | Some (Build_Resp cm im dm) =>
+                               let (am, descQm, dtQm) := reqFn cm im in
+                                 d = dtQm /\ am = a /\ descQm = St /\
+                                 forall t', tm < t' < t -> noStore respFn t' a
+                           | None => False
+                         end.
 
-  Record FirstLevel :=
-    {
-      latestValue:
-        forall t a pCache,
-          let p := node pCache in
-          clean a t p ->
-          (data (s t) p a = initData a /\
-           forall t', t' < t -> noStore (respFn cl) t' a ) \/
-          (exists tm,
-             tm < t /\
-             match respFn cl tm with
-               | Some (Build_Resp cm im dm) =>
-                 let (am, descQm, dtQm) := reqFn cm im in
-                 data (s t) p a = dtQm /\ am = a /\ descQm = St /\
-                 forall t', tm < t' < t -> noStore (respFn cl) t' a
-               | None => False
-             end);
+  Parameter latestValue:
+    forall t a pCache,
+      let p := node pCache in
+      clean a t p ->
+      noStoreData (data t p a) a t \/ isStoreData (data t p a) a t.
 
-      processReq:
-        forall t, 
-        match respFn cl t with
-          | Some (Build_Resp cProc _ _) =>
-            let c := p_node cProc in
-            let (a, op, d) := reqFn cProc (next (s t) c) in
-            match op with
-              | Ld => sle coh (Sh coh) (state (s t) c a)
-              | St => state (s t) c a = Mo coh
-            end
-          | None => True
-        end;
+  Parameter processReq:
+    forall t, 
+      match respFn t with
+        | Some (Build_Resp cProc _ _) =>
+          let c := p_node cProc in
+          let (a, op, d) := reqFn cProc (next t c) in
+          match op with
+            | Ld => le Sh (state t c a)
+            | St => state t c a = Mo
+          end
+        | None => True
+      end.
+   
+  Parameter nextChange:
+    forall t p,
+      let c := p_node p in
+      next (S t) c <> next t c ->
+      match respFn t with
+        | Some (Build_Resp cProc' _ _) => p_node cProc' = c
+        | None => False
+      end.
+   
+  Parameter noReqAgain:
+    forall t,
+    match respFn t with
+      | Some (Build_Resp cProc _ _) =>
+        let c := p_node cProc in
+        next (S t) c = S (next t c)
+      | None => True
+    end.
+End FirstLevel.
 
-      nextChange:
-        forall t p,
-          let c := p_node p in
-          next (nextS t) c <> next (s t) c ->
-          match respFn cl t with
-            | Some (Build_Resp cProc' _ _) => p_node cProc' = c
-            | None => False
-          end;
-
-      noReqAgain:
-        forall t,
-        match respFn cl t with
-          | Some (Build_Resp cProc _ _) =>
-            let c := p_node cProc in
-            next (nextS t) c = S (next (s t) c)
-          | None => True
-        end
-    }.
-
-  Section Addr.
+Module mkStoreAtomic (Import coh: Coherence) (Import cl: CacheLocal coh) (Import fl: FirstLevel coh cl).
+  Section ForAddr.
     Variable a: Addr.
-
-    Variable fl: FirstLevel.
-
     Lemma nextIncOrSame:
       forall t p,
         let c := p_node p in
-        next (getCacheState cl t) c = next (getCacheState cl (S t)) c \/
-        next (getCacheState cl (S t)) c = S (next (getCacheState cl t) c).
+        next t c = next (S t) c \/
+        next (S t) c = S (next t c).
     Proof.
       intros t p c.
-      expandClFl cl fl.
-      assert (opts: next (getCacheState t) c = next (getCacheState (S t)) c \/
-                    next (getCacheState (S t)) c <> next (getCacheState t) c) by omega.
-      specialize (nextChange t p).
-      specialize (noReqAgain t).
+      assert (opts: next t c = next (S t) c \/
+                    next (S t) c <> next t c) by omega.
+      pose proof (@nextChange t p) as nextChange.
+      pose proof (noReqAgain t) as noReqAgain.
       destruct opts; repeat destructAll;
       try match goal with
-            | [H: (next (getCacheState (S t)) c <> next (getCacheState t) c) |- _ ] =>
-                specialize (nextChange H); rewrite nextChange in *
+            | [H: (next (S t) c <> next t c) |- _ ] =>
+                specialize (nextChange H); try rewrite nextChange in *
           end;
       intuition.
     Qed.
 
     Lemma increasingIdx: forall t1 t2, t1 <= t2 -> forall p,
                                                      let c := p_node p in
-                                                     next (s t1) c <=
-                                                     next (s t2) c.
+                                                     next t1 c <=
+                                                     next t2 c.
     Proof.
       intros t1 t2 cond p c.
       diff t1 t2 cond.
-      unfold s in *.
       induction td; simplArith.
       omega.
       destruct (nextIncOrSame (t1 + td) p) as [eq|neq]; unfold c in *; omega.
     Qed.
 
-    Lemma incrOnResp: forall t1 t2, t1 < t2 -> match respFn cl t1 with
+    Lemma incrOnResp: forall t1 t2, t1 < t2 -> match respFn t1 with
                                                  | Some (Build_Resp c1 i1 _) =>
-                                                   next (s t2) (p_node c1) > i1
+                                                   next t2 (p_node c1) > i1
                                                  | _ => True
                                                end.
     Proof.
       intros t1 t2 t1_lt_t2.
       assert (St1_le_t2: S t1 <= t2) by omega.
       pose proof (increasingIdx St1_le_t2) as u1.
-      unfold s in *.
-      expandClFl cl fl.
-      specialize (noReqAgain t1).
-      specialize (respFnIdx t1).
+      pose proof (noReqAgain t1).
+      pose proof (respFnIdx t1).
       repeat destructAll;
-        match goal with
-          | [c: Proc |- _] => specialize (u1 c); omega
+        repeat match goal with
+          | c: Proc |- _ => specialize (u1 c); omega
           | _ => intuition
         end.
     Qed.
 
     Theorem uniqRespLabels':
-      forall t1 t2, match respFn cl t1, respFn cl t2 with
+      forall t1 t2, match respFn t1, respFn t2 with
                       | Some (Build_Resp c1 i1 _), Some (Build_Resp c2 i2 _) =>
                         p_node c1 = p_node c2 -> i1 = i2 -> t1 = t2
                       | _, _ => True
                     end.
     Proof.
-      Ltac finish incrOnResp respFnIdx t2 lt :=
-        specialize (incrOnResp _ _ lt);
+      Ltac finish incrOnResp respFnIdx t2 slt :=
+        specialize (incrOnResp _ _ slt);
         specialize (respFnIdx t2);
         repeat destructAll;
         match goal with
-          | [|- True] => intuition
-          | _ => try (intros pEq idEq; rewrite pEq, idEq in *; omega)
+          | _ => intros pEq idEq; rewrite pEq, idEq in *; omega
+          | _ => intuition
         end.
 
       intros t1 t2.
       pose proof @incrOnResp as incr;
       assert (opts: t1 = t2 \/ t1 < t2 \/ t2 < t1) by (unfold Time in *; omega).
-      expandClFl cl fl.
-      destruct opts as [eq| [lt|gt]].
+      destruct opts as [eq| [slt|sgt]].
       repeat destructAll; intuition.
-      finish incr respFnIdx t2 lt.
-      finish incr respFnIdx t1 gt.
+      finish incr respFnIdx t2 slt.
+      finish incr respFnIdx t1 sgt.
     Qed.
 
     Theorem localOrdering':
-      forall t1 t2, match respFn cl t1, respFn cl t2 with
+      forall t1 t2, match respFn t1, respFn t2 with
                       | Some (Build_Resp c1 i1 _), Some (Build_Resp c2 i2 _) =>
                         p_node c1 = p_node c2 -> i1 > i2 -> t1 > t2
                       | _, _ => True
@@ -173,24 +145,23 @@ Section FirstLevel.
       destruct opts as [lt|le].
       repeat destructAll; intuition.
       pose proof (increasingIdx le) as incr.
-      unfold s, nextS in *.
-      expandCl cl.
       pose proof (respFnIdx t1) as r1.
       pose proof (respFnIdx t2) as r2.
       repeat destructAll; intros;
-      match goal with
-        | [H: p_node ?p1 = p_node ?p2 |- _] => rewrite H in *;
-                                               specialize (incr p2); omega
-        | _ => intuition
-      end.
+        repeat match goal with
+                 | [H: p_node ?p1 = p_node ?p2 |- _] =>
+                     rewrite H in *;
+                             specialize (incr p2); omega
+                 | _ => intuition
+               end.
     Qed.
 
     Lemma allPrevIdx:
       forall t2 p2 i1,
         let c2 := p_node p2 in
-        i1 < next (getCacheState cl t2) c2 ->
+        i1 < next t2 c2 ->
         exists t1, t1 < t2 /\
-                   match respFn cl t1 with
+                   match respFn t1 with
                      | Some (Build_Resp c1 i _) =>
                          p_node c1 = c2 /\ i = i1
                      | None => False
@@ -204,23 +175,22 @@ Section FirstLevel.
 
       intros t2 p2 i1 c2 i1LtNext.
       induction t2.
-      rewrite nextZero in *; omega.
+      rewrite next0 in *; omega.
       unfold c2 in *.
       pose proof (nextIncOrSame t2 p2) as opts.
-      expandClFl cl fl.
       destruct opts as [same | inc].
       rewrite same in *.
       finishPrev IHt2 t2 i1LtNext.
 
-      assert (opts: i1 < next (getCacheState t2) (p_node p2) \/ i1 = next (getCacheState t2) (p_node p2))
+      assert (opts: i1 < next t2 (p_node p2) \/ i1 = next t2 (p_node p2))
              by omega;
       destruct opts as [lt | same].
       finishPrev IHt2 t2 lt.
 
       rewrite same in *.
-      assert (ne: next (getCacheState (S t2)) (p_node p2) <> next (getCacheState t2) (p_node p2)) by omega.
-      specialize (nextChange t2 p2 ne).
-      specialize (respFnIdx t2).
+      assert (ne: next (S t2) (p_node p2) <> next t2 (p_node p2)) by omega.
+      pose proof (nextChange p2 ne).
+      pose proof (respFnIdx t2).
       exists t2.
       repeat destructAll; try omega; match goal with
                                        | [H: p_node ?p = p_node p2 |- _ ] => rewrite <- H in *; intuition
@@ -228,10 +198,10 @@ Section FirstLevel.
     Qed.
 
     Theorem allPrevious':
-      forall t2, match respFn cl t2 with
+      forall t2, match respFn t2 with
                    | Some (Build_Resp c2 i2 _) =>
                        forall i1, i1 < i2 -> exists t1, t1 < t2 /\
-                                                           match respFn cl t1 with
+                                                           match respFn t1 with
                                                              | Some (Build_Resp c1 i _) =>
                                                                  p_node c1 = p_node c2 /\ i = i1
                                                              | None => False
@@ -240,19 +210,16 @@ Section FirstLevel.
                  end.
     Proof.
       intros t2.
-      pose proof (allPrevIdx t2) as u1.
-      expandClFl cl fl.
-      specialize (respFnIdx t2).
+      pose proof (@allPrevIdx t2) as u1.
+      pose proof (respFnIdx t2).
       repeat destructAll;
       try match goal with
             | [p: Proc |- _] => specialize (u1 (p_node p))
           end; intuition.
     Qed.
-  End Addr.
+  End ForAddr.
 
   Section Sa.
-    Variable fl: FirstLevel.
-
     Lemma leafProp: forall p c, ~ parent c (node (proc p)).
     Proof.
       unfold not; intros p c c_p.
@@ -263,11 +230,11 @@ Section FirstLevel.
     Qed.
 
     Lemma cleanProp:
-      forall t p coh loc,
-        sle coh (Sh coh) (state (getCacheState cl t) (node (proc p)) loc) ->
-        sle coh (Sh coh) (state (getCacheState cl t) (node (proc p)) loc) /\
+      forall t p loc,
+        le Sh (state t (node (proc p)) loc) ->
+        le Sh (state t (node (proc p)) loc) /\
         (forall c, parent c (node (proc p)) ->
-                   sle coh (dir (getCacheState cl t) (node (proc p)) c loc) (Sh coh)).
+                   le (dir t (node (proc p)) c loc) Sh).
     Proof.
       intros.
       pose proof (leafProp p) as leafProp.
@@ -280,41 +247,32 @@ Section FirstLevel.
 
     Theorem storeAtomicity':
       forall t,
-        match respFn cl t with
+        match respFn t with
           | Some (Build_Resp c i d) =>
             let (a, descQ, dtQ) := reqFn c i in
             match descQ with
               | Ld =>
-                (d = initData a /\ forall t', t' < t -> noStore (respFn cl) t' a) \/
-                (exists tm,
-                   tm < t /\
-                   match respFn cl tm with
-                     | Some (Build_Resp cm im dm) =>
-                       let (am, descQm, dtQm) := reqFn cm im in
-                       d = dtQm /\ am = a /\ descQm = St /\
-                       forall t', tm < t' < t -> noStore (respFn cl) t' a
-                     | _ => False
-                   end)
-              | St => d = initData zero 
+                  noStoreData d a t \/ isStoreData d a t
+              | St => d = initData zero
             end
           | _ => True
         end.
     Proof.
       intros t.
-      pose proof (cleanProp t) as cleanProp.
-      expandClFl cl fl.
-      specialize (respFnIdx t).
-      specialize (respFnLdData t).
-      specialize (latestValue t).
-      specialize (processReq t).
-      unfold p_node in respFnLdData.
+      unfold noStoreData, isStoreData.
+      pose proof (@cleanProp t) as cleanProp.
+      pose proof (respFnIdx t) as respFnIdx.
+      pose proof (respFnLdData t) as respFnLdData.
+      pose proof (@latestValue t).
+      pose proof (processReq t) as processReq.
+      unfold p_node in *.
       destructAll.
       destructAll.
-      rewrite <- respFnIdx in processReq.
+      rewrite <- respFnIdx in *.
       destructAll.
       destructAll.
 
-      specialize (latestValue loc (proc procR) (cleanProp _ _ _ processReq));
+      specialize (latestValue (proc procR) (cleanProp _ _ processReq));
       simpl in *; rewrite <- respFnLdData in *;
       intuition.
 
@@ -323,10 +281,10 @@ Section FirstLevel.
       intuition.
     Qed.
 
-    Theorem fullStoreAtomicity: StoreAtomicity (respFn cl).
+    Theorem fullStoreAtomicity: StoreAtomicity respFn.
     Proof.
-      apply (Build_StoreAtomicity (respFn cl) (uniqRespLabels' fl) (localOrdering' fl)
-                                  (allPrevious' fl) storeAtomicity').
+      apply (Build_StoreAtomicity respFn uniqRespLabels' localOrdering'
+                                  allPrevious' storeAtomicity').
     Qed.
   End Sa.
-End FirstLevel.
+End mkStoreAtomic.
