CacheLocal.v
@@ -2,6 +2,50 @@ Require Import DataTypes Coherence Tree.
 
 Set Implicit Arguments.
 
+Module Type CacheLocal (Import coh: Coherence).
+  Parameter state: Time -> Tree -> Addr -> t.
+  Parameter dir: Time -> Tree -> Tree -> Addr -> t.
+  Parameter data: Time -> Tree -> Addr -> Data.
+  Parameter wait: Time -> Tree -> Addr -> bool.
+  Parameter waitS: Time -> Tree -> Addr -> t.
+  Parameter dwait: Time -> Tree -> Tree -> Addr -> bool.
+  Parameter dwaitS: Time -> Tree -> Tree -> Addr -> t.
+  Parameter next: Time -> Tree -> nat.
+
+  Parameter respFn: Time -> option Resp.
+
+  Parameter respFnIdx: forall t,
+                         match respFn t with
+                           | Some (Build_Resp c i _) => i = next t (p_node c)
+                           | None => True
+                         end.
+  Parameter respFnLdData: forall t,
+                            match respFn t with
+                              | Some (Build_Resp c i d) =>
+                                  match desc (reqFn c i) with
+                                    | Ld => d = data t (p_node c) (loc (reqFn c i))
+                                    | St => d = initData zero
+                                  end
+                              | None => True
+                            end.
+
+  Parameter state0: state 0 = fun c a =>
+                                match decTree c hier with
+                                  | left _ => Mo
+                                  | right _ => In
+                                end.
+
+  Parameter dir0: dir 0 = fun p c a => In.
+
+  Parameter data0: data 0 = fun c a => initData a.
+
+  Parameter wait0: wait 0 = fun c a => false.
+
+  Parameter dwait0: dwait 0 = fun p c a => false.
+
+  Parameter next0: next 0 = fun c => 0.
+End CacheLocal.
+(*
 Section CacheLocal.
   Variable State: Set.
 
@@ -35,19 +79,6 @@ Section CacheLocal.
       dwaitZero: dwait (getCacheState 0) = fun p c a => false;
       nextZero: next (getCacheState 0) = fun c => 0;
 
-      respFnIdx: forall t,
-                   match respFn t with
-                     | Some (Build_Resp c i _) => i = next (getCacheState t) (p_node c)
-                     | None => True
-                   end;
-      respFnLdData: forall t,
-                      match respFn t with
-                        | Some (Build_Resp c i d) =>
-                          match desc (reqFn c i) with
-                            | Ld => d = data (getCacheState t) (p_node c) (loc (reqFn c i))
-                            | St => d = initData zero
-                          end
-                        | None => True
-                      end
     }.
 End CacheLocal.
+*)
